intermediate/Veritas.Intermediate.TSLog.fsti
@@ -1,13 +1,20 @@
 module Veritas.Intermediate.TSLog
 
 open Veritas.Interleave
+open Veritas.SeqAux
 open Veritas.State
 open Veritas.Intermediate.Global
 open Veritas.Intermediate.Logs
+open Veritas.Intermediate.Store
+open Veritas.Intermediate.Verify
 
 module I = Veritas.Interleave
+module SA = Veritas.SeqAux
+module SpecTS = Veritas.Verifier.TSLog
 module IntL = Veritas.Intermediate.Logs
 module IntG = Veritas.Intermediate.Global
+module IntT = Veritas.Intermediate.Thread
+module IntV = Veritas.Intermediate.Verify
 
 let il_logS vcfg = interleaving (logS_entry vcfg)
 
@@ -37,6 +44,24 @@ val lemma_prefix_verifiable (#vcfg:_) (itsl: its_log vcfg) (i:nat{i <= I.length 
   Lemma (ensures (verifiable (I.prefix itsl i) /\ clock_sorted (I.prefix itsl i)))
         [SMTPat (I.prefix itsl i)]
 
+let thread_id_of #vcfg (il: its_log vcfg) (i: I.seq_index il): valid_tid il =
+  fst (I.i2s_map il i)
+
+let thread_state #vcfg (il:its_log vcfg)
+                 (tid:valid_tid il)
+  : Tot (vs:vtls vcfg{Valid? vs}) = 
+  let gs = g_logS_of il in
+  let tl = IntG.thread_log gs tid in
+  IntT.verify tl
+
+let thread_state_pre #vcfg (il: its_log vcfg) (i: I.seq_index il): (vs:vtls vcfg{Valid? vs}) = 
+  let tid = thread_id_of il i in
+  thread_state (I.prefix il i) tid
+
+let thread_state_post #vcfg (il: its_log vcfg) (i: I.seq_index il): (vs:vtls vcfg{Valid? vs}) = 
+  let tid = thread_id_of il i in
+  thread_state (I.prefix il (i + 1)) tid
+
 let lemma_logS_interleave_implies_state_ops_interleave #vcfg (l: logS vcfg) (gl: g_logS vcfg{interleave #(logS_entry vcfg) l gl})
   : Lemma (interleave #state_op (IntL.to_state_ops l) (IntG.to_state_ops gl)) 
   = FStar.Squash.bind_squash
@@ -46,3 +71,85 @@ let lemma_logS_interleave_implies_state_ops_interleave #vcfg (l: logS vcfg) (gl:
       (fun i -> 
         let i' = filter_map_interleaving is_state_op to_state_op i in
         FStar.Squash.return_squash i')
+
+let same_shape #a #b (il:I.interleaving a) (il':I.interleaving b) =
+  let open I in
+  let IL s ss _ = il in
+  let IL s' ss' _ = il' in
+  Seq.length s == Seq.length s' /\
+  Seq.length ss == Seq.length ss' /\
+  (forall (i:SA.seq_index ss). Seq.length (Seq.index ss i) == Seq.length (Seq.index ss i))
+
+val to_logk (#vcfg:_) (il:its_log vcfg) 
+  : Tot (sil:SpecTS.il_vlog { same_shape il sil })
+
+val lemma_to_logk_length (#vcfg:_) (il:its_log vcfg)
+  : Lemma (ensures I.length il = I.length (to_logk il))
+          [SMTPat (to_logk il)]
+
+val lemma_to_logk_thread_count (#vcfg:_) (il:its_log vcfg)
+  : Lemma (ensures thread_count il = SpecTS.thread_count (to_logk il))
+          [SMTPat (to_logk il)]
+
+val lemma_to_logk_thread_id_of (#vcfg:_) (il:its_log vcfg) (i:I.seq_index il)
+  : Lemma (ensures thread_id_of il i == SpecTS.thread_id_of (to_logk il) i)
+          [SMTPat (SpecTS.thread_id_of (to_logk il) i)]
+
+val lemma_to_logk_prefix_commute (#vcfg:_) (il:its_log vcfg) (i:nat{i <= I.length il})
+  : Lemma (to_logk (I.prefix il i) == I.prefix (to_logk il) i)
+
+val lemma_its_log_valid_step (#vcfg:_) (il:its_log vcfg) (i:I.seq_index il)
+  : Lemma (ensures Valid? (IntV.verify_step (thread_state_pre il i) (I.index il i)))
+          [SMTPat (thread_state_pre il i)]
+
+(* after processing il, the thread store of every verifier thread is a map *)
+let forall_store_ismap #vcfg (il:its_log vcfg)
+  = forall (tid:valid_tid il). 
+    {:pattern (thread_store (thread_state il tid))}
+      is_map (thread_store (thread_state il tid))
+
+(* 
+ * if all the stores are maps before entry i and the store after processing entry i step is a map, then 
+ * all stores are maps after entry i 
+ *)
+val lemma_forall_store_ismap_extend (#vcfg:_) (il:its_log vcfg) (i:I.seq_index il)
+  : Lemma (requires (forall_store_ismap (I.prefix il i) /\ 
+                     is_map (thread_store (thread_state_post il i))))
+          (ensures (forall_store_ismap (I.prefix il (i + 1))))
+
+(* the intermediate and spec level verifier states correspond to one-another after processing 
+ * il and il', respectively *)
+let forall_vtls_rel #vcfg (il:its_log vcfg) (il':SpecTS.il_vlog) 
+  = thread_count il = SpecTS.thread_count il' /\
+    (forall (tid:valid_tid il). 
+      {:pattern vtls_rel (thread_state il tid) (SpecTS.thread_state il' tid)}
+       vtls_rel (thread_state il tid) (SpecTS.thread_state il' tid))
+
+val lemma_forall_vtls_rel_extend (#vcfg:_) (ils:its_log vcfg) (i:I.seq_index ils)
+  : Lemma (requires (let ils_i = I.prefix ils i in
+                     let ilk = to_logk ils in
+                     let ilk_i = I.prefix ilk i in                     
+                     forall_vtls_rel ils_i ilk_i /\
+                     vtls_rel (thread_state_post ils i) 
+                              (SpecTS.thread_state_post ilk i)))
+          (ensures (let ilk = to_logk ils in
+                    let ils_i1 = I.prefix ils (i + 1) in
+                    let ilk_i1 = I.prefix ilk (i + 1) in
+                    forall_vtls_rel ils_i1 ilk_i1))
+
+val lemma_forall_vtls_rel_implies_spec_verifiable (#vcfg:_) (ils:its_log vcfg)
+  : Lemma (requires (let ilk = to_logk ils in
+                     forall_vtls_rel ils ilk))
+          (ensures (let ilk = to_logk ils in
+                    SpecTS.verifiable ilk))
+          [SMTPat (forall_vtls_rel ils (to_logk ils))]
+
+(*
+val lemma_vtls_rel_implies_spec_clock_sorted (#vcfg:_) (ils:its_log vcfg)
+  : Lemma (requires (let ilk = to_logk ils in
+                     forall_vtls_rel (I.prefix il i) (I.prefix il' i)  /\
+                     forall_vtls_rel (I.prefix il (i + 1)) (I.prefix il' (i + 1)) /\
+                     SpecTS.clock_sorted (I.prefix il' i)))
+          (ensures (let il' = ilogS_to_logK il in
+                    SpecTS.clock_sorted (I.prefix il' (i + 1))))
+*)
